\documentclass{article}
\usepackage[utf8]{inputenc}
\usepackage[english]{babel}
\usepackage{amsfonts}
\usepackage{amsthm}
\usepackage{amsmath}
\usepackage{amssymb}

\newtheorem{theorem}{Theorem}
\newtheorem{es}{Examples}

\begin{document}
    \textbf{P3}.
    Let $R$ and $S$ be regular expressions, then consider the statement: If $R^{*} \equiv S^{*}$, then $R \equiv S$.\\
    We prove this is false. Consider the counterexample:\\
    Let $R = 0$ and $S = 0^{*}$. We obtain the result that $R^{*}\equiv S^{*}$ by the property of \textit{idempotence} of the
    Kleene star. However, it is not true that $R \equiv S$ since the empty string would be in the language generated by $S$
    but not in the language generated by $R$.\\

\end{document}
